src/Verification.v
@@ -4,6 +4,7 @@ Require Import Assembly.
 Require Import Simulation.
 Require Import Compiler.
 Require Import List.
+Require Import Lia.
 Import ListNotations.
 Require Import PeanoNat.
 Import Nat.
@@ -11,11 +12,16 @@ Module Verification.
 Inductive compile : Language.state -> Assembly.state -> Prop :=
   | comp_r : forall p a, Compiler.compile p = Some a -> compile p a.
 
+Definition eval := Language.semantics.
+Definition eval' := Assembly.semantics.
+
 Theorem comp_correct : 
-  Simulation.plus_forward_sim compile Language.semantics Assembly.semantics.
+  Simulation.plus_forward_sim compile eval eval'.
 Proof.
   unfold Simulation.plus_forward_sim.
-  intros.
+  induction p.
+
+    
 Admitted. (* to be done. *)
 
 End Verification.
